Add comments.

Liveness.v
@@ -5,6 +5,9 @@ Set Implicit Arguments.
 
 Local Hint Resolve incl_empty minus_incl incl_right incl_left.
 
+(** * Liveness *)
+
+(** We have two flavors of liveness: functional and imperative. See comments in inductive definition [live_sound]. *)
 
 Inductive overapproximation : Set
   := Functional | Imperative | FunctionalAndImperative.
@@ -23,72 +26,7 @@ Definition isImperative (o:overapproximation) :=
     | _ => false
   end.
 
-Inductive argsLive (Caller Callee:set var) : args -> params -> Prop :=
-| AL_nil : argsLive Caller Callee nil nil
-| AL_cons y z Y Z
-  : argsLive Caller Callee Y Z
-    -> (z ∈ Callee -> live_exp_sound y Caller)
-    -> argsLive Caller Callee (y::Y) (z::Z).
-
-Lemma argsLive_length lv bv Y Z
-  : argsLive lv bv Y Z
-  -> length Y = length Z.
-Proof.
-  intros. general induction H; simpl; eauto.
-Qed.
-
-Lemma argsLive_liveSound lv blv Y Z
-: argsLive lv blv Y Z
-  -> forall (n : nat) (y : exp),
-      get (filter_by (fun y : var => B[y ∈ blv]) Z Y) n y ->
-      live_exp_sound y lv.
-Proof.
-      intros. general induction H; simpl in * |- *.
-      - isabsurd.
-      - decide (z ∈ blv); eauto.
-        inv H1; eauto.
-Qed.
-
-Lemma argsLive_live_exp_sound lv blv Y Z y z n
-: argsLive lv blv Y Z
-  -> get Y n y
-  -> get Z n z
-  -> z ∈ blv
-  -> live_exp_sound y lv.
-Proof.
-  intros. general induction n; inv H0; inv H1; inv H; intuition; eauto.
-Qed.
-
-Lemma argsLive_agree_on' (V E E':onv val) lv blv Y Z v v'
-:  argsLive lv blv Y Z
- -> agree_on eq lv E E'
- -> omap (exp_eval E) Y = Some v
- -> omap (exp_eval E') Y = Some v'
- -> agree_on eq blv (V [Z <-- List.map Some v]) (V [Z <-- List.map Some v']).
-Proof.
-  intros. general induction H; simpl in * |- *; eauto.
-  - monad_inv H2. monad_inv H3.
-    decide (z ∈ blv).
-    +erewrite <- exp_eval_live in EQ0; eauto.
-     *  assert (x1 = x) by congruence.
-        subst. simpl.
-        eauto using agree_on_update_same, agree_on_incl.
-    + eapply agree_on_update_dead_both; eauto.
-Qed.
-
-Lemma argsLive_agree_on (V V' E E':onv val) lv blv Y Z v v'
-: agree_on eq (blv \ of_list Z) V V'
-  -> argsLive lv blv Y Z
-  -> agree_on eq lv E E'
-  -> omap (exp_eval E) Y = Some v
-  -> omap (exp_eval E') Y = Some v'
-  -> agree_on eq blv (V [Z <-- List.map Some v]) (V' [Z <-- List.map Some v']).
-Proof.
-  intros. etransitivity; eauto using argsLive_agree_on'.
-  eapply update_with_list_agree; eauto.
-  exploit omap_length; eauto. exploit argsLive_length; eauto.
-  rewrite map_length; congruence.
-Qed.
+(** ** Inductive Definition of Liveness *)
 
 Inductive live_sound (i:overapproximation) : list (set var*params) -> stmt -> ann (set var) -> Prop :=
 | LOpr x Lv b lv e (al:ann (set var))
@@ -105,7 +43,7 @@ Inductive live_sound (i:overapproximation) : list (set var*params) -> stmt -> an
   -> getAnn al2 ⊆ lv
   -> live_sound i Lv (stmtIf e b1 b2) (ann2 lv al1 al2)
 | LGoto l Y Lv lv blv Z
-  : get Lv (counted l) (blv,Z)
+  : get Lv (counted l) (blv,Z) (** Imperative Liveness requires the globals of a function to be live at the call site *)
   -> (if isImperative i then ((blv \ of_list Z) ⊆ lv) else True)
   -> length Y = length Z
   -> (forall n y, get Y n y -> live_exp_sound y lv)
@@ -122,11 +60,13 @@ Inductive live_sound (i:overapproximation) : list (set var*params) -> stmt -> an
 | LLet Lv s Z b lv als alb
   : live_sound i ((getAnn als,Z)::Lv) s als
   -> live_sound i ((getAnn als,Z)::Lv) b alb
-  -> (of_list Z) ⊆ getAnn als
+  -> (of_list Z) ⊆ getAnn als  (** Functional Liveness requires the globals of a function to be live at the definition (for building the closure) *)
   -> (if isFunctional i then (getAnn als \ of_list Z ⊆ lv) else True)
   -> getAnn alb ⊆ lv
   -> live_sound i Lv (stmtFun Z s b)(ann2 lv als alb).
 
+
+(** ** Relation between different overapproximations *)
 
 Lemma live_sound_overapproximation_I Lv s slv
 : live_sound FunctionalAndImperative Lv s slv -> live_sound Imperative Lv s slv.
@@ -140,11 +80,14 @@ Proof.
   intros. general induction H; simpl in * |- *; econstructor; simpl; eauto.
 Qed.
 
+(** ** [live_sound] ensures that the annotation matches the program *)
 Lemma live_sound_annotation i Lv s slv
 : live_sound i Lv s slv -> annotation s slv.
 Proof.
   intros. general induction H; econstructor; eauto.
 Qed.
+
+(** ** Some monotonicity properties *)
 
 Definition live_ann_subset (lvZ lvZ' : set var * list var) :=
   match lvZ, lvZ' with
@@ -190,6 +133,8 @@ Proof.
     cset_tac; intuition.
 Qed.
 
+(** ** Live variables always contain the free variables *)
+
 Lemma freeVars_live s lv Lv
   : live_sound Functional Lv s lv -> IL.freeVars s ⊆ getAnn lv.
 Proof.
@@ -211,6 +156,8 @@ Proof.
     rewrite IHlive_sound1; eauto.
     rewrite IHlive_sound2; eauto.
 Qed.
+
+(** ** Liveness is stable under renaming *)
 
 Definition live_rename_L_entry (ϱ:env var) (x:set var * params)
  := (lookup_set ϱ (fst x), lookup_list ϱ (snd x)).
@@ -269,6 +216,8 @@ Proof.
     destruct i; simpl; eauto; eapply lookup_set_incl; eauto.
     eapply lookup_set_incl; eauto.
 Qed.
+
+(** ** For functional programs, only free variables are significant *)
 
 Inductive approxF :  F.block -> F.block -> Prop :=
  | approxFI E E' Z s
@@ -344,6 +293,8 @@ Proof.
     eapply agree_on_incl; eauto.
 Qed.
 
+(** ** Since live variables contain free variables, liveness contains all variables significant to an IL/F program *)
+
 Inductive approxF' : list (set var * params) -> F.block -> F.block -> Prop :=
   approxFI' DL E E' Z s lv
   : live_sound Functional ((getAnn lv, Z)::DL) s lv
@@ -371,6 +322,7 @@ Proof.
   eapply agree_on_incl; eauto. eapply freeVars_live; eauto.
 Qed.
 
+(** ** Live variables contain all variables significant to an IL/I program *)
 
 Inductive approxI
   : list (set var * params) -> I.block -> I.block -> Prop :=
